Merge in current progress on monadic refinement proof (#5)
* Non-monadic cases

* progress in Current_memory

* adding the invariant

* partial cleanup from misguided attempts

* Hoare triple proof for Current_memory

* Hoare triple proof for Get_local + trivial cases solved

* Progress on more cases + failure on Call_indirect

* Set_local done

* call indirect complete + simplification

* set_global + cleanup

* attempt at Invoke

* Invoke finished

* cleanup

Authored-by: Maja Trela <maja.ada0@gmail.com>

WebAssembly/Wasm_Interpreter_Monad_Properties.thy
@@ -153,18 +153,8 @@ qed
   term app_s_f_v_s_mem_size_m
 term app_s_f_v_s_mem_size
 
-definition "mem_m_assn \<equiv> \<lambda>(mr,mm) (mri,mmi). mri \<mapsto>\<^sub>b\<^sub>a Rep_mem_rep mr * \<up>(mmi=mm)"
 
-definition "inst_m_assn i ii \<equiv> 
-    inst_m.types ii \<mapsto>\<^sub>a inst.types i
-  * inst_m.funcs ii \<mapsto>\<^sub>a inst.funcs i  
-  * inst_m.tabs  ii \<mapsto>\<^sub>a inst.tabs  i 
-  * inst_m.mems  ii \<mapsto>\<^sub>a inst.mems  i 
-  * inst_m.globs ii \<mapsto>\<^sub>a inst.globs i"
-     
-lemma [sep_heap_rules]: "<mem_m_assn m mi> len_byte_array (fst mi) <\<lambda>r. mem_m_assn m mi * \<up>(r=length (Rep_mem_rep (fst m)))>"
-  unfolding mem_m_assn_def
-  by (sep_auto split: prod.splits)
+definition "mem_m_assn \<equiv> \<lambda>(mr,mm) (mr_m,mm_m). mr_m \<mapsto>\<^sub>b\<^sub>aRep_mem_rep mr * \<up>(mm_m=mm)"
 
 method extract_list_idx for i :: nat =
   (subst listI_assn_extract[of i], (simp;fail), (simp;fail))
@@ -174,43 +164,568 @@ method reinsert_list_idx for i :: nat =
   (frame_inference; fail),
   (simp;fail),
   (simp;fail)
+
+method knock_down for i :: nat = 
+ extract_pre_pure?, extract_list_idx i, sep_auto, extract_pre_pure?, reinsert_list_idx i
+
+term app_s_f_v_s_mem_size_m
+term app_s_f_v_s_mem_size
+
+
+definition "inst_m_assn i i_m \<equiv> 
+    inst_m.types i_m \<mapsto>\<^sub>a inst.types i
+  * inst_m.funcs i_m \<mapsto>\<^sub>a inst.funcs i  
+  * inst_m.tabs  i_m \<mapsto>\<^sub>a inst.tabs  i 
+  * inst_m.mems  i_m \<mapsto>\<^sub>a inst.mems  i 
+  * inst_m.globs i_m \<mapsto>\<^sub>a inst.globs i"
+
+lemma [sep_heap_rules]: "<mem_m_assn m mi> len_byte_array (fst mi) 
+<\<lambda>r. mem_m_assn m mi * \<up>(r=length (Rep_mem_rep (fst m)))>"
+  unfolding mem_m_assn_def
+  by (sep_auto split: prod.splits)
+
+type_synonym inst_store = "(inst list \<times> inst_m list)"
+
+abbreviation "inst_store_assn \<equiv> \<lambda>(is, i_ms). list_assn inst_m_assn is i_ms"
+
+abbreviation "inst_at \<equiv> \<lambda>(is, i_ms) (i, i_m) j. j < length is \<and> is!j = i \<and> i_ms!j = i_m"
+
+abbreviation "contains_inst_assn i_s i \<equiv> \<exists>\<^sub>A j. \<up>(inst_at i_s i j)"
+
+definition mems_m_assn :: "mem list \<Rightarrow> mem_m array \<Rightarrow> assn" where
+  "mems_m_assn ms ms_m = (\<exists>\<^sub>A ms_i. ms_m \<mapsto>\<^sub>a ms_i  * list_assn mem_m_assn ms ms_i)"
+
+definition cl_m_assn :: "inst_store \<Rightarrow> cl \<Rightarrow> cl_m \<Rightarrow> assn" where 
+  "cl_m_assn i_s cl cl_m = (case cl of 
+  cl.Func_native i tf ts b_es \<Rightarrow> 
+    (case cl_m of 
+    cl_m.Func_native i_m tf_m ts_m b_es_m \<Rightarrow> 
+     contains_inst_assn i_s (i, i_m) * \<up>(tf = tf_m \<and> ts = ts_m \<and> b_es = b_es_m) 
+  | cl_m.Func_host tf_m host_m \<Rightarrow> false)
+| cl.Func_host tf host \<Rightarrow> 
+    (case cl_m of 
+    cl_m.Func_native i_m tf_m ts_m b_es_m \<Rightarrow> false 
+  | cl_m.Func_host tf_m host_m \<Rightarrow> \<up>(tf = tf_m \<and> host = host_m))
+)"
+
+lemma ex_assn_pure_conv:"(\<exists>\<^sub>Ax. \<up>(P x)) = \<up>(\<exists>x. P x)"
+  by (smt (z3) ent_ex_preI ent_iffI ent_pure_pre_iff_sng ent_refl triv_exI)
+
+lemma cl_m_assn_pure:"is_pure_assn (cl_m_assn i_s cl cl_m)"
+  unfolding cl_m_assn_def 
+  by(simp split: cl.split cl_m.split add:ex_assn_pure_conv)
   
-lemma "< mi \<mapsto>\<^sub>a mis * (list_assn mem_m_assn) ms mis * inst_m_assn (f_inst i) ii > 
-    app_s_f_v_s_mem_size_m mi ii vs 
-  <\<lambda>r. \<up>(r = app_s_f_v_s_mem_size ms i vs) *
-   mi \<mapsto>\<^sub>a mis * (list_assn mem_m_assn) ms mis * inst_m_assn (f_inst i) ii>"
+
+lemma cl_m_assn_type:
+  assumes "h \<Turnstile> cl_m_assn i_s cl cl_m" 
+  shows "cl_type cl = cl_m_type cl_m"
+  using assms
+  unfolding cl_m_assn_def cl_type_def cl_m_type_def
+  by(simp split:cl.splits cl_m.splits)
+
+definition funcs_m_assn :: "inst_store \<Rightarrow> cl list \<Rightarrow> cl_m array \<Rightarrow> assn" where
+  "funcs_m_assn i_s fs fs_m = (\<exists>\<^sub>A fs_i. fs_m \<mapsto>\<^sub>a fs_i * list_assn (cl_m_assn i_s) fs fs_i)"
+
+definition tabinst_m_assn :: "tabinst \<Rightarrow> tabinst_m \<Rightarrow> assn" where 
+  "tabinst_m_assn = (\<lambda>(tr,tm) (tr_m,tm_m). tr_m \<mapsto>\<^sub>a tr * \<up>(tm = tm_m))"
+
+definition tabs_m_assn :: "tabinst list \<Rightarrow> tabinst_m array \<Rightarrow> assn" where
+ "tabs_m_assn ts ts_m = (\<exists>\<^sub>A ts_i. ts_m \<mapsto>\<^sub>a ts_i * list_assn tabinst_m_assn ts ts_i)"
+
+definition "globs_m_assn gs gs_m \<equiv> gs_m \<mapsto>\<^sub>a gs"
+
+definition s_m_assn :: "inst_store \<Rightarrow> s \<Rightarrow> s_m \<Rightarrow> assn" where 
+  "s_m_assn i_s s s_m = 
+  funcs_m_assn i_s (s.funcs s) (s_m.funcs s_m)
+* tabs_m_assn  (s.tabs s)  (s_m.tabs s_m)
+* mems_m_assn  (s.mems s)  (s_m.mems s_m)
+* globs_m_assn (s.globs s) (s_m.globs s_m)"
+
+definition locs_m_assn :: "v list \<Rightarrow> v array \<Rightarrow> assn" where 
+  "locs_m_assn locs locs_m = locs_m \<mapsto>\<^sub>a locs"
+
+definition fc_m_assn :: "inst_store \<Rightarrow> frame_context \<Rightarrow> frame_context_m \<Rightarrow> assn" where 
+  "fc_m_assn i_s fc fc_m = (
+  case fc of Frame_context redex lcs nf f \<Rightarrow> 
+  case fc_m of Frame_context_m redex_m lcs_m nf_m f_locs1 f_inst2 \<Rightarrow>
+  \<up>(redex = redex_m \<and> lcs = lcs_m \<and> nf = nf_m)
+  * contains_inst_assn i_s (f_inst f, f_inst2)
+  * locs_m_assn (f_locs f) f_locs1
+)"
+
+definition "fcs_m_assn i_s fcs fcs_m \<equiv> list_assn (fc_m_assn i_s) fcs fcs_m"
+
+lemma [simp]:"fcs_m_assn i_s (fc#fcs) (fc_m#fcs_m) = 
+  fc_m_assn i_s fc fc_m * fcs_m_assn i_s fcs fcs_m"
+  unfolding fcs_m_assn_def by simp
+
+definition cfg_m_assn :: "inst_store \<Rightarrow> config \<Rightarrow> config_m \<Rightarrow> assn" where
+  "cfg_m_assn i_s cfg cfg_m = (
+  case cfg of Config d s fc fcs \<Rightarrow>
+  case cfg_m of Config_m d_m s_m fc_m fcs_m \<Rightarrow> 
+  \<up>(d=d_m) * s_m_assn i_s s s_m * fc_m_assn i_s fc fc_m * fcs_m_assn i_s fcs fcs_m
+   * inst_store_assn i_s
+)"     
+
+lemma mem_size_triple:
+  assumes "inst_at (is, i_ms) (f_inst f, f_inst2) j" 
+  shows 
+  "< ms_m \<mapsto>\<^sub>a ms_i * list_assn mem_m_assn ms ms_i * inst_store_assn (is, i_ms) > 
+    app_s_f_v_s_mem_size_m ms_m f_inst2 v_s 
+  <\<lambda>r. \<up>(r = app_s_f_v_s_mem_size ms f v_s) *
+   ms_m \<mapsto>\<^sub>a ms_i * (list_assn mem_m_assn) ms ms_i * inst_store_assn (is, i_ms)>"
+  using assms
   unfolding app_s_f_v_s_mem_size_m_def inst_m_assn_def list_assn_conv_idx
-  apply extract_pre_pure
   apply sep_auto
-  apply (extract_list_idx "inst.mems (f_inst i) ! 0")
-  apply (sep_auto)
-  apply (reinsert_list_idx "inst.mems (f_inst i) ! 0")
-  apply (sep_auto)
-  subgoal by (auto simp add: app_s_f_v_s_mem_size_def smem_ind_def mem_size_def mem_length_def mem_rep_length_def split: option.split list.split)  
+   apply (knock_down j)
+  apply(sep_auto)
+  apply(knock_down "inst.mems (f_inst f) ! 0")
+   apply (sep_auto)
+  subgoal by (auto simp add: app_s_f_v_s_mem_size_def smem_ind_def mem_size_def 
+        mem_length_def mem_rep_length_def split: option.split list.split)  
   apply (sep_auto)
   done
-    
+
+
+
+lemma get_local_triple: 
+  "<locs_m_assn (f_locs f) f_locs1> 
+  app_f_v_s_get_local_m k f_locs1 v_s 
+  <\<lambda>r. \<up>(r = app_f_v_s_get_local k f v_s) * locs_m_assn (f_locs f) f_locs1>"
+  unfolding locs_m_assn_def app_f_v_s_get_local_m_def app_f_v_s_get_local_def
+  by sep_auto
+
+
+lemma get_global_triple:
+  assumes "inst_at (is, i_ms) (f_inst f, f_inst2) j"
+  shows "<globs_m_assn gs gs_m * inst_store_assn (is, i_ms)>
+  app_s_f_v_s_get_global_m k gs_m f_inst2 v_s
+  <\<lambda>r.\<up>(r = app_s_f_v_s_get_global k gs f v_s)
+  * globs_m_assn gs gs_m * inst_store_assn (is, i_ms)>"
+  using assms
+  unfolding globs_m_assn_def inst_m_assn_def app_s_f_v_s_get_global_m_def app_s_f_v_s_get_global_def
+    sglob_ind_def list_assn_conv_idx
+  apply (sep_auto)
+   apply (knock_down j)
+  apply (sep_auto)
+  done
+
+lemma set_local_triple: 
+  assumes "inst_at (is, i_ms) (f_inst f, f_inst2) j"
+  shows "<locs_m_assn (f_locs f) f_locs1 * inst_store_assn (is, i_ms)> 
+  app_f_v_s_set_local_m k f_locs1 v_s
+  <\<lambda>r. let (f', v_s', res) = (app_f_v_s_set_local k f v_s) in 
+  \<up>(r = (v_s', res) \<and> inst_at (is, i_ms) (f_inst f', f_inst2) j) 
+  * locs_m_assn (f_locs f') f_locs1 * inst_store_assn (is, i_ms)>"
+  using assms
+  unfolding locs_m_assn_def app_f_v_s_set_local_m_def app_f_v_s_set_local_def
+  by(sep_auto)
+
+
+(*unfortunately I have to phrase it as (is, i_ms), otherwise sep_auto gets confused*)
+lemma set_global_triple: 
+  assumes "inst_at (is, i_ms) (f_inst f, f_inst2) j"
+  shows "<globs_m_assn gs gs_m * inst_store_assn (is, i_ms)> 
+  app_s_f_v_s_set_global_m k gs_m f_inst2 v_s
+  <\<lambda>r. let (gs', v_s', res) = (app_s_f_v_s_set_global k gs f v_s) in 
+  \<up>(r = (v_s', res)) 
+  * globs_m_assn gs' gs_m * inst_store_assn (is, i_ms)>"
+  using assms
+  unfolding app_s_f_v_s_set_global_m_def inst_m_assn_def globs_m_assn_def list_assn_conv_idx
+  apply (sep_auto simp: app_s_f_v_s_set_global_def update_glob_def sglob_ind_def Let_def
+      split: prod.split)
+   apply (knock_down j)
+  apply(sep_auto)
+  done
+
+
+(* app_s_f_v_s_set_global_def update_glob_def sglob_ind_def Let_def *)
+
+lemma call_triple: 
+  assumes "inst_at (is, i_ms) (f_inst f, f_inst2) j"
+  shows
+ "<inst_store_assn (is, i_ms)> 
+  app_f_call_m k f_inst2 
+  <\<lambda>r. \<up>(r = app_f_call k f) * inst_store_assn (is, i_ms)>"
+  using assms
+  unfolding inst_m_assn_def app_f_call_m_def app_f_call_def sfunc_ind_def list_assn_conv_idx
+  apply(sep_auto)
+   apply(knock_down j)
+  apply(sep_auto)
+  done
+
+
+lemmas is_complex_goal = asm_rl[of "< _ > _ < _ >"] asm_rl[of "_ \<Longrightarrow>\<^sub>A _"]
+
+method_setup then_else = \<open>let
+in
+  Method.text_closure -- Method.text_closure -- Method.text_closure >>
+    (fn ((textb, textt), texte) => fn ctxt => fn using => fn st =>
+      let
+        val bmethod = Method.evaluate_runtime textb ctxt using;
+        val tmethod = Method.evaluate_runtime textt ctxt using;
+        val emethod = Method.evaluate_runtime texte ctxt using;
+      in
+        (case try (fn st => bmethod st |> Seq.pull) st of
+          SOME (SOME (Seq.Result st,_)) => tmethod st
+        | _ => emethod st)
+      end)
+end     
+\<close>
+
+method defer_vcg = then_else \<open>rule is_complex_goal\<close> \<open>fail\<close> 
+  \<open>find_goal \<open>rule is_complex_goal\<close>, 
+  (rule is_complex_goal | tactic \<open>defer_tac 1\<close>)\<close>
+
+method sep_auto_all = (defer_vcg | (rule is_complex_goal, sep_auto))+
+
+lemma [sep_heap_rules]: "<tabinst_m_assn t t_m> 
+    Array.len (fst t_m) 
+    <\<lambda>r. tabinst_m_assn t t_m * \<up>(r=length (fst t))>"
+  unfolding tabinst_m_assn_def
+  by (sep_auto split: prod.splits)
+
+lemma [sep_heap_rules]: "<tabinst_m_assn t t_m> 
+    Array.nth (fst t_m) x
+    <\<lambda>r. tabinst_m_assn t t_m * \<up>(r=(fst t)!x)>"
+  unfolding tabinst_m_assn_def
+  by (sep_auto split: prod.splits)
+
+lemma funcs_nth_type_triple:"<funcs_m_assn i_s cls cls_m> 
+    Array.nth cls_m i  
+    <\<lambda>r. \<up>(cl_m_type r = cl_type (cls!i)) * funcs_m_assn i_s cls cls_m>" 
+  unfolding funcs_m_assn_def list_assn_conv_idx
+  apply(sep_auto heap del:nth_rule)
+  apply(extract_pre_pure)
+  apply(sep_auto)
+  apply(simp add: listI_assn_extract[of i])
+  using cl_m_assn_type 
+  by (metis mod_starD)
+
+lemma call_indirect_triple:
+  assumes "inst_at (is, i_ms) (f_inst f, f_inst2) j"
+  shows 
+  "<tabs_m_assn ts ts_m * funcs_m_assn i_s fs fs_m * inst_store_assn (is, i_ms)> 
+  app_s_f_v_s_call_indirect_m k ts_m fs_m f_inst2 v_s
+  <\<lambda>r. \<up>(r = app_s_f_v_s_call_indirect k ts fs f v_s) 
+* tabs_m_assn ts ts_m * funcs_m_assn i_s fs fs_m * inst_store_assn (is, i_ms)>"
+  using assms
+  unfolding app_s_f_v_s_call_indirect_m_def 
+  supply [split] = v.splits option.splits
+  apply(sep_auto)
+  unfolding inst_m_assn_def tabs_m_assn_def list_assn_conv_idx
+   apply(sep_auto_all)
+       apply(knock_down j)
+      apply sep_auto_all
+      apply(knock_down "inst.tabs (f_inst f) ! 0")
+      apply(sep_auto_all)
+      apply(knock_down "inst.tabs (f_inst f) ! 0")
+       apply(sep_auto_all)
+         apply(sep_auto heap: funcs_nth_type_triple)
+        apply(sep_auto_all)
+         apply(knock_down j)
+        apply(sep_auto_all)
+         apply(simp_all add:app_s_f_v_s_call_indirect_def Let_def split:list.splits)
+     apply(auto simp add:stypes_def tab_cl_ind_def)
+  done
+
+
 find_theorems app_s_f_v_s_mem_size
 
-lemma run_step_b_e_m_run_step_b_e_Unreachable:
-  assumes "execute (run_step_b_e_m Unreachable cfg_m) h = Some ((cfg_m', res), h')"
-  shows "run_step_b_e Unreachable (config_m_to_config h cfg_m) = ((config_m_to_config h' cfg_m'), res)"
-  using assms
-  by (auto simp add: Heap_Monad.return_def Heap_Monad.heap_def config_m_to_config_def split: frame_context_m.splits frame_context.splits config_m.splits redex.splits prod.splits)
+lemmas splits = 
+  frame_context_m.splits frame_context.splits config.splits config_m.splits redex.splits prod.splits
 
-lemma run_step_b_e_m_run_step_b_e:
-  assumes "execute (run_step_b_e_m b_e cfg_m) h = Some ((cfg_m', res), h')"
-  shows "run_step_b_e b_e (config_m_to_config h cfg_m) = ((config_m_to_config h' cfg_m'), res)"
-  using assms
+lemmas defs =  
+  Heap_Monad.return_def Heap_Monad.heap_def 
+  config_m_to_config_def frame_context_m_to_frame_context_def
+
+
+abbreviation cfg_m_pair_assn where 
+  "cfg_m_pair_assn i_s p p_m \<equiv> 
+  let (cfg, res) = p in 
+  let (cfg_m, res_m) = p_m in 
+  cfg_m_assn i_s cfg cfg_m * \<up>(res = res_m)"
+
+  
+lemma run_step_b_e_m_triple:
+    "<cfg_m_assn i_s cfg cfg_m> 
+    run_step_b_e_m b_e cfg_m 
+    <\<lambda>r. cfg_m_pair_assn i_s (run_step_b_e b_e cfg) r>\<^sub>t"
+proof - 
+  obtain d s fc fcs where config:"cfg = Config d s fc fcs"
+    by(erule config.exhaust)
+  obtain redex lcs nf f where frame:"fc = Frame_context redex lcs nf f" 
+    by(erule frame_context.exhaust)
+  obtain v_s es b_es where redex:"redex = Redex v_s es b_es" 
+    by(erule redex.exhaust)
+
+  obtain d_m s_m fc_m fcs_m where config_m:"cfg_m = Config_m d_m s_m fc_m fcs_m" 
+    by(erule config_m.exhaust)  
+  obtain redex_m lcs_m nf_m f_locs1 f_inst2 
+    where frame_m:"fc_m = Frame_context_m redex_m lcs_m nf_m f_locs1 f_inst2" 
+    by(erule frame_context_m.exhaust)
+  obtain v_s_m es_m b_es_m where redex_m:"redex_m = Redex v_s_m es_m b_es_m" 
+    by(erule redex.exhaust)
+
+  note unfold_vars_m = config_m frame_m redex_m
+
+  note unfold_vars = config frame redex unfold_vars_m
+
+  note unfold_vars_assns = unfold_vars cfg_m_assn_def fc_m_assn_def
+
+  show ?thesis
+  proof (cases b_e)
+    case (Tee_local k)
+    then show ?thesis unfolding unfold_vars_assns by sep_auto
+  next
+    case (Set_global k)
+    then show ?thesis unfolding unfold_vars_assns s_m_assn_def 
+      (*comment on instability*)
+      by (sep_auto heap:set_global_triple split:prod.splits)
+  next
+    case (Load t tp_sx a off)
+    then show ?thesis sorry
+  next
+    case (Store t tp a off)
+    then show ?thesis sorry
+  next
+    case Grow_memory
+    then show ?thesis sorry
+  next
+    case Current_memory
+    then show ?thesis 
+      unfolding unfold_vars_assns s_m_assn_def mems_m_assn_def 
+      by(sep_auto heap:mem_size_triple split:prod.splits)
+  next
+    case (Set_local k)
+    then show ?thesis 
+      unfolding unfold_vars_assns
+      by (sep_auto heap: set_local_triple[of _ _ f f_inst2] split:prod.splits)
+  next
+    case (Get_local k)
+    then show ?thesis 
+      unfolding unfold_vars_assns by (sep_auto heap:get_local_triple)
+  next
+    case (Get_global k)
+    then show ?thesis 
+      unfolding unfold_vars_assns s_m_assn_def by (sep_auto heap:get_global_triple split:prod.splits)
+  next
+    case (Call k)
+    then show ?thesis 
+      unfolding unfold_vars_assns by (sep_auto heap:call_triple split:prod.splits)
+  next
+    case (Call_indirect k)
+    then show ?thesis 
+      unfolding unfold_vars_assns s_m_assn_def by (sep_auto heap:call_indirect_triple split:prod.splits)
+  next
+    case Return (* this case relies on garbage collection *)
+
+    show ?thesis
+      unfolding Return unfold_vars_assns fcs_m_assn_def
+      by (sep_auto split:splits list.split)
+  next
+    case (Block tf b_ebs)
+    then show ?thesis unfolding unfold_vars_assns by(sep_auto split:tf.splits)
+  next
+    case (Loop tfs b_els)
+    then show ?thesis unfolding unfold_vars_assns by(sep_auto split:tf.splits)
+  next
+    case (Br k)
+    then show ?thesis unfolding unfold_vars_assns by(sep_auto split:label_context.splits)
+  next
+    case Unreachable
+    then show ?thesis unfolding unfold_vars_assns by sep_auto
+  next
+    case Nop
+    then show ?thesis unfolding unfold_vars_assns by sep_auto
+  next
+    case Drop 
+    then show ?thesis unfolding unfold_vars_assns by sep_auto
+  next
+    case Select 
+    then show ?thesis unfolding unfold_vars_assns by sep_auto
+  next
+    case (If tf es1 es2) 
+    then show ?thesis unfolding unfold_vars_assns by sep_auto
+  next
+    case (Br_if k)
+    then show ?thesis unfolding unfold_vars_assns by sep_auto
+  next
+    case (Br_table ks k)
+    then show ?thesis unfolding unfold_vars_assns by sep_auto
+  next
+    case (EConst k)
+    then show ?thesis unfolding unfold_vars_assns by sep_auto
+  next
+    case (Unop t op)
+    then show ?thesis unfolding unfold_vars_assns by sep_auto
+  next
+    case (Binop t op)
+    then show ?thesis unfolding unfold_vars_assns by sep_auto
+  next
+    case (Testop t op)
+    then show ?thesis unfolding unfold_vars_assns by sep_auto
+  next
+    case (Relop t op)
+    then show ?thesis unfolding unfold_vars_assns by sep_auto
+  next
+    case (Cvtop t2 op t1 sx)
+    then show ?thesis unfolding unfold_vars_assns by sep_auto
+  qed
+qed
+
+abbreviation "s_m_vs_pair_assn i_s \<equiv> \<lambda>(s, vs) (s_m, vs_m). s_m_assn i_s s s_m * \<up>(vs=vs_m)"
+
+abbreviation "s_m_vs_opt_assn i_s a a_m s s_m \<equiv> (case a of 
+   Some s_vs \<Rightarrow> (case a_m of Some s_vs_m \<Rightarrow> s_m_vs_pair_assn i_s s_vs s_vs_m | None \<Rightarrow> false) 
+ | None \<Rightarrow> (case a_m of Some s_vs_m \<Rightarrow> false | None \<Rightarrow> s_m_assn i_s s s_m)) "
+
+lemma host_apply_impl_m_triple:
+ "< s_m_assn i_s s s_m>
+ host_apply_impl_m s_m tf h vs
+ <\<lambda>r. s_m_vs_opt_assn i_s (host_apply_impl s tf h vs) r s s_m>"
   sorry
+
+lemma host_apply_impl_m_triple':
+ "< funcs_m_assn i_s (s.funcs s) (s_m.funcs s_m) 
+* tabs_m_assn (s.tabs s) (s_m.tabs s_m) * mems_m_assn (s.mems s) (s_m.mems s_m) 
+* globs_m_assn (s.globs s) (s_m.globs s_m)>
+ host_apply_impl_m s_m tf h vs
+ <\<lambda>r. s_m_vs_opt_assn i_s (host_apply_impl s tf h vs) r s s_m>"
+  sorry
+
+lemma host_apply_impl_m_triple'':
+ "< s_m.funcs s_m \<mapsto>\<^sub>a fs_i * list_assn (cl_m_assn i_s) (s.funcs s) fs_i
+* tabs_m_assn (s.tabs s) (s_m.tabs s_m) * mems_m_assn (s.mems s) (s_m.mems s_m) 
+* globs_m_assn (s.globs s) (s_m.globs s_m)>
+ host_apply_impl_m s_m tf h vs
+ <\<lambda>r. s_m_vs_opt_assn i_s (host_apply_impl s tf h vs) r s s_m>"
+  sorry
+
+
+lemma ent_triple_preI:
+  assumes "\<And>h. h\<Turnstile>P \<Longrightarrow> P \<Longrightarrow>\<^sub>A Q"
+  shows "P \<Longrightarrow>\<^sub>A Q"
+  using assms unfolding entails_def by auto
+
+method extract_pre_pure' uses dest =
+  (rule hoare_triple_preI | rule ent_triple_preI | drule asm_rl[of "_\<Turnstile>_"]),
+  (determ \<open>elim mod_starE dest[elim_format] extract_pure_rules[elim_format]\<close>)?,
+  ((determ \<open>thin_tac "_ \<Turnstile> _"\<close>)+)?,
+  (simp (no_asm) only: triv_forall_equality)?
+
+lemma pure_dup:
+  assumes "is_pure_assn P" 
+  shows "P = P*P" 
+  using assms unfolding is_pure_assn_def
+  by auto
+
+
+lemma [sep_heap_rules]:
+  "< fs_m\<mapsto>\<^sub>a fs_i * list_assn (cl_m_assn i_s) fs fs_i> 
+  Array.nth fs_m i 
+  <\<lambda>r. \<up>(i < length fs_i \<and> r = fs_i!i) 
+  * cl_m_assn i_s (fs!i) r * fs_m \<mapsto>\<^sub>a fs_i * list_assn (cl_m_assn i_s) fs fs_i>"
+  unfolding funcs_m_assn_def list_assn_conv_idx 
+  apply(sep_auto)
+  apply(extract_pre_pure')
+  apply(extract_list_idx i)
+  apply(subst pure_dup[OF cl_m_assn_pure])
+  apply(reinsert_list_idx i)
+  apply(sep_auto)
+  done
+
+
+lemma run_step_e_m_triple:
+    "<cfg_m_assn i_s cfg cfg_m> 
+    run_step_e_m e cfg_m 
+    <\<lambda>r. cfg_m_pair_assn i_s (run_step_e e cfg) r>\<^sub>t"
+proof -
+  obtain d s fc fcs where config:"cfg = Config d s fc fcs"
+    by(erule config.exhaust)
+  obtain redex lcs nf f where frame:"fc = Frame_context redex lcs nf f" 
+    by(erule frame_context.exhaust)
+  obtain v_s es b_es where redex:"redex = Redex v_s es b_es" 
+    by(erule redex.exhaust)
+  obtain d_m s_m fc_m fcs_m where config_m:"cfg_m = Config_m d_m s_m fc_m fcs_m" 
+    by(erule config_m.exhaust)  
+  obtain redex_m lcs_m nf_m f_locs1 f_inst2 
+    where frame_m:"fc_m = Frame_context_m redex_m lcs_m nf_m f_locs1 f_inst2" 
+    by(erule frame_context_m.exhaust)
+  obtain v_s_m es_m b_es_m where redex_m:"redex_m = Redex v_s_m es_m b_es_m" 
+    by(erule redex.exhaust)
+  note unfold_vars_m = config_m frame_m redex_m
+  note unfold_vars = config frame redex unfold_vars_m
+  note unfold_vars_assns = unfold_vars cfg_m_assn_def fc_m_assn_def
+
+  show ?thesis 
+  proof (cases e)
+    case (Basic b_e)
+    have 1:"run_step_e_m (Basic b_e) cfg_m = run_step_b_e_m b_e cfg_m"
+      unfolding unfold_vars_m by simp
+    have 2:"run_step_e (Basic b_e) cfg = run_step_b_e b_e cfg"
+      unfolding unfold_vars by simp 
+    show ?thesis unfolding Basic 1 2 by(sep_auto heap:run_step_b_e_m_triple)
+  next
+    case (Invoke i_cl)
+
+    show ?thesis unfolding Invoke unfold_vars_assns 
+      supply [simp] = Let_def and 
+        [split] = splits v.splits option.splits cl.splits cl_m.splits tf.splits nat.splits
+      and [sep_heap_rules] = host_apply_impl_m_triple''
+      apply(sep_auto simp:s_m_assn_def funcs_m_assn_def heap del: nth_rule)
+      supply [simp] = cl_m_assn_def locs_m_assn_def s_m_assn_def funcs_m_assn_def fc_m_assn_def 
+                apply(sep_auto_all)
+      apply (sep_auto)
+      done
+  next
+    case Trap
+    then show ?thesis unfolding unfold_vars by sep_auto
+  next
+    case (Label x41 x42 x43)
+    then show ?thesis unfolding unfold_vars by sep_auto
+  next
+    case (Frame x51 x52 x53)
+    then show ?thesis unfolding unfold_vars by sep_auto
+  qed
+qed 
 
 lemma run_step_e_m_run_step_e:
-  assumes "execute (run_step_e_m e cfg_m) h = Some ((cgf_m', res), h')"
-  shows "run_step_e e (config_m_to_config h cfg_m) = ((config_m_to_config h' cfg_m'), res)"
-  sorry
+  assumes 
+    "execute (run_step_e_m e cfg_m) h = Some ((cfg_m', res), h')"
+  shows 
+    "run_step_e e (config_m_to_config h cfg_m) = ((config_m_to_config h' cfg_m'), res)"
+proof(cases e)
+  case (Basic b_e)
+  have 1:"run_step_e_m e cfg_m = run_step_b_e_m b_e cfg_m" unfolding Basic
+    by(rule config_m.induct, auto simp add: defs split: splits)
+  have "run_step_e e (config_m_to_config h cfg_m) = run_step_b_e b_e (config_m_to_config h cfg_m)"
+    unfolding Basic by(rule config.induct, auto simp add: defs split: splits) 
+  also have "... = ((config_m_to_config h' cfg_m'), res)" 
+    using assms sorry
+  finally show ?thesis by -
+next
+  case (Invoke i_cl)
+  then show ?thesis sorry
+next
+  case Trap
+  show ?thesis using assms by (auto simp add: defs Trap split: splits)
+next
+  case (Label x41 x42 x43)
+  show ?thesis using assms by (auto simp add: defs Label split: splits)
+next
+  case (Frame x51 x52 x53)
+  show ?thesis using assms by (auto simp add: defs Frame split: splits)
+qed
 
 lemma run_iter_m_run_iter:
-  assumes "execute (run_iter_m n cfg_m) h = Some ((cgf_m', res), h')"
-  shows "run_iter n (config_m_to_config h cfg_m) = ((config_m_to_config h' cfg_m'), res)"
-  sorry
+  "execute (run_iter_m n cfg_m) h = Some ((cfg_m', res), h')
+ \<Longrightarrow> run_iter n (config_m_to_config h cfg_m) = ((config_m_to_config h' cfg_m'), res)"
+proof(induct n)
+  case 0
+  show ?case using 0 by (auto simp add: defs split: splits)
+next
+  case (Suc n)
+  then show ?case sorry
+qed
 end
